MoonbitSemantics/Mcore/PrimTyping.lean
@@ -85,5 +85,7 @@ theorem evalPrim_type_sound'
       | tuple hvts => cases op <;> simp [evalPrim] at heval <;> simp [typeOfPrim] at hprim <;> subst_vars <;> first | exact .unit | exact .tuple hvts
       | locConstr => cases op <;> simp [evalPrim] at heval <;> simp [typeOfPrim] at hprim <;> subst_vars <;> first | exact .unit | exact .locConstr
       | locArray => cases op <;> simp [evalPrim] at heval <;> simp [typeOfPrim] at hprim <;> subst_vars <;> first | exact .unit | exact .locArray
+      | errorValueResultOk hvt => cases op <;> simp [evalPrim] at heval <;> simp [typeOfPrim] at hprim <;> subst_vars <;> first | exact .unit | exact .errorValueResultOk hvt
+      | errorValueResultErr hvt => cases op <;> simp [evalPrim] at heval <;> simp [typeOfPrim] at hprim <;> subst_vars <;> first | exact .unit | exact .errorValueResultErr hvt
 
 end Moonbit.Mcore
